Added runtime check that destination addresses of direct messages are good. (If invariants are carried forward from previous states, this was already know in this case. But we want to guarantee this property even if code is not proved correct.)

smc-next/Forwarding.ec
@@ -28,8 +28,8 @@ theory FwDir_.
    functionality: pt1 is asking to forward u to pt2 *)
 
 type fw_req =
-  {fw_req_func : addr;   (* address of functionality *)
-   fw_req_pt1  : port;   (* source = port requesting forwarding *)
+  {fw_req_func : addr;   (* address of functionality - destination address *)
+   fw_req_pt1  : port;   (* port requesting forwarding - source address *)
    (* data: *)
    fw_req_pt2  : port;   (* port being forwarded to *)
    fw_req_u    : univ}.  (* universe value to be forwarded *)
@@ -106,8 +106,8 @@ qed.
    requested by pt1 *)
 
 type fw_rsp =
-  {fw_rsp_func : addr;   (* address of functionality *)
-   fw_rsp_pt2  : port;   (* destination = port being forwarded to *)
+  {fw_rsp_func : addr;   (* address of functionality - source address *)
+   fw_rsp_pt2  : port;   (* port being forwarded to - destination address *)
    (* data: *)
    fw_rsp_pt1  : port;   (* port requesting forwarding *)
    fw_rsp_u    : univ}.  (* universe value to be forwarded *)
@@ -196,8 +196,8 @@ theory FwAdv.
    pt2 on behalf of pt1 *)
 
 type fw_obs =
-  {fw_obs_func : addr;   (* address of functionality *)
-   fw_obs_adv  : addr;   (* address of adversary *)
+  {fw_obs_func : addr;   (* address of functionality - source address *)
+   fw_obs_adv  : addr;   (* address of adversary - destination address *)
    (* data: *)
    fw_obs_pt1  : port;   (* port requesting forwarding *)
    fw_obs_pt2  : port;   (* port being forwarded to *)
@@ -276,8 +276,8 @@ qed.
    proceed with forwarding *)
 
 type fw_ok =
-  {fw_ok_func : addr;   (* address of functionality *)
-   fw_ok_adv  : addr    (* address of adversary *)
+  {fw_ok_func : addr;   (* address of functionality - destination address *)
+   fw_ok_adv  : addr    (* address of adversary - source address *)
    (* data: (none) *)
   }.
 
@@ -356,6 +356,10 @@ module Forw : FUNC = {
     self <- self_; adv <- adv_; st <- FwStateInit;
   }
 
+  (* we insert sufficient checks for target and source addresses
+     of sent messages to be valid; depending upon the invariants
+     maintained, some of them will be redundant *)
+
   proc parties(m : msg) : msg option = {
     var r : msg option <- None;
     match st with
@@ -367,11 +371,13 @@ module Forw : FUNC = {
             if (envport self adv x.`FwDir.D.fw_req_pt2) {
               r <-
                 Some
-                (FwAdv.epdp_fw_obs_msg.`enc
-                 {|FwAdv.fw_obs_func = self; FwAdv.fw_obs_adv = adv;
-                   FwAdv.fw_obs_pt1 = x.`FwDir.D.fw_req_pt1;
-                   FwAdv.fw_obs_pt2 = x.`FwDir.D.fw_req_pt2;
-                   FwAdv.fw_obs_u = x.`FwDir.D.fw_req_u|});
+                (FwAdv.epdp_fw_obs_msg.`enc   (* adversarial message *)
+                 {|FwAdv.fw_obs_func = self;  (* source address *)
+                   FwAdv.fw_obs_adv  = adv;   (* destination address *)
+                   (* data: *)
+                   FwAdv.fw_obs_pt1  = x.`FwDir.D.fw_req_pt1;
+                   FwAdv.fw_obs_pt2  = x.`FwDir.D.fw_req_pt2;
+                   FwAdv.fw_obs_u    = x.`FwDir.D.fw_req_u|});
               st <-
                 FwStateWait x.`FwDir.D.fw_req_pt1 x.`FwDir.D.fw_req_pt2
                 x.`FwDir.D.fw_req_u;
@@ -383,13 +389,20 @@ module Forw : FUNC = {
     | FwStateWait pt1 pt2 u => {
         match FwAdv.epdp_fw_ok_msg.`dec m with
           Some x => {
-            (* x.`FwAdv.fw_ok_func = self /\ x.`FwAdv.fw_ok_adv = adv *)
-            r <-
-              Some
-              (FwDir.D.epdp_fw_rsp_msg.`enc
-               {|FwDir.D.fw_rsp_func = self; FwDir.D.fw_rsp_pt1 = pt1;
-                 FwDir.D.fw_rsp_pt2 = pt2; FwDir.D.fw_rsp_u = u|});
-            st <- FwStateFinal;
+            (* x.`FwAdv.fw_ok_func = self /\ x.`FwAdv.fw_ok_adv = adv;
+               if the invariant from FwInitState is preserved, the
+               following test is redudant: *)
+            if (envport self adv pt2) {
+              r <-
+                Some
+                (FwDir.D.epdp_fw_rsp_msg.`enc   (* direct message *)
+                 {|FwDir.D.fw_rsp_func = self;  (* source address *)
+                   FwDir.D.fw_rsp_pt2  = pt2;   (* destination address *)
+                   (* data: *)
+                   FwDir.D.fw_rsp_pt1  = pt1;
+                   FwDir.D.fw_rsp_u    = u|});
+              st <- FwStateFinal;
+            }
           }
         | None => { }
         end;
@@ -476,6 +489,8 @@ move => pt1 pt2 u pt1' pt2' u'.
 match => //.
 auto.
 move => x x'.
+if => //.
+auto.
 auto.
 auto.
 qed.
@@ -504,7 +519,8 @@ lemma Forw_invoke_init_fw_req (m' : msg) :
       FwAdv.fw_obs_u    = fwr.`FwDir.D.fw_req_u|}) /\
    Forw.st =
      FwStateWait fwr.`FwDir.D.fw_req_pt1 fwr.`FwDir.D.fw_req_pt2
-     fwr.`FwDir.D.fw_req_u] = 1%r.
+     fwr.`FwDir.D.fw_req_u /\
+   envport Forw.self Forw.adv fwr.`FwDir.D.fw_req_pt2] = 1%r.
 proof.
 proc.
 sp 1.
@@ -541,16 +557,19 @@ auto.
 auto.
 qed.
 
-pred forw_invoke_wait_fw_ok (self adv : addr, m : msg) =
+pred forw_invoke_wait_fw_ok (self adv : addr, pt2 : port, m : msg) =
   is_valid FwAdv.epdp_fw_ok_msg m /\
   (oget (FwAdv.epdp_fw_ok_msg.`dec m)).`FwAdv.fw_ok_func = self /\
-  (oget (FwAdv.epdp_fw_ok_msg.`dec m)).`FwAdv.fw_ok_adv = adv.
+  (oget (FwAdv.epdp_fw_ok_msg.`dec m)).`FwAdv.fw_ok_adv = adv /\
+  (oget (FwAdv.epdp_fw_ok_msg.`dec m)).`FwAdv.fw_ok_func = self /\
+  envport self adv pt2.
 
 lemma Forw_invoke_wait_fw_ok (st' : fw_state, m' : msg) :
   phoare
   [Forw.invoke :
    st' = Forw.st /\ m' = m /\ get_as_FwStateWait Forw.st <> None /\
-   forw_invoke_wait_fw_ok Forw.self Forw.adv m ==>
+   forw_invoke_wait_fw_ok Forw.self Forw.adv
+   (oget (get_as_FwStateWait Forw.st)).`2 m ==>
    let wait = oget (get_as_FwStateWait st') in
    res =
    Some
@@ -565,11 +584,14 @@ rcondt 1; first auto; smt(FwAdv.eq_of_valid_fw_ok).
 inline Forw.parties.
 sp 2.
 match FwStateWait 1.
-auto => /> &hr.
+auto => |> &hr.
 rewrite /get_as_FwStateWait.
 case (Forw.st{hr}) => // pt1 pt2 u /= _.
 by exists pt1 pt2 u.
-match Some 1; first auto; smt().
+match Some 1; first auto => |> &hr.
+rewrite /get_as_FwStateWait /= /#.
+rcondt 1; first auto => |> &hr _ _.
+by rewrite /forw_invoke_wait_fw_ok /get_as_FwStateWait.
 auto; by rewrite /get_as_FwStateWait.
 qed.
 
@@ -577,7 +599,8 @@ lemma Forw_invoke_wait_bad (st' : fw_state) :
   phoare
   [Forw.invoke :
    st' = Forw.st /\ get_as_FwStateWait Forw.st <> None /\
-   ! forw_invoke_wait_fw_ok Forw.self Forw.adv m ==>
+   ! forw_invoke_wait_fw_ok Forw.self Forw.adv
+     (oget (get_as_FwStateWait Forw.st)).`2 m ==>
    res = None /\ Forw.st = st'] = 1%r.
 proof.
 proc.
@@ -594,8 +617,12 @@ case (FwAdv.epdp_fw_ok_msg.`dec m0 = None).
 match None 1; first auto.
 auto.
 match Some 1.
-auto; smt().
-exfalso; smt(FwAdv.eq_of_valid_fw_ok).
+auto; progress.
+exists (oget (FwAdv.epdp_fw_ok_msg.`dec m{hr})).
+by apply some_oget.
+if.
+exfalso; smt(oget_some FwAdv.eq_of_valid_fw_ok).
+auto.
 auto.
 qed.
 
